# Chapter exercises
## Semigroup exercises
Given a datatype, implement the Semigroup instance. Add Semigroup constraints to type variables where needed.  

Use the Semigroup class from **base** or write your own. When we use `<>`, we mean the infix `mappend` operation from the Semigroup type class.

*Note We’re not always going to derive every instance you may want or need in the datatypes we provide for exercises. We expect you to know what you need and to take care of it yourself by this point.*  

1. Validate all of your instances with `QuickCheck`. Since the only law is **associativity**, that’s the only property you need to reuse. Keep in mind that you’ll potentially need to import the modules for Monoid and Semigroup and to avoid naming conflicts for <>, depending on your version of GHC:  

data Trivial = Trivial deriving (Eq, Show)  

instance Semigroup Trivial where  
_ <> _ = undefined  
instance Arbitrary Trivial where  
arbitrary = return Trivial  
semigroupAssoc :: (Eq m, Semigroup m)  
=> m -> m -> m -> Bool  
semigroupAssoc a b c =  
(a <> (b <> c)) == ((a <> b) <> c)  
type TrivAssoc =  
Trivial -> Trivial -> Trivial -> Bool  
main :: IO ()  
main =  
quickCheck (semigroupAssoc :: TrivAssoc)  

> What I Learnt:
- semigroup association cannot be applied to Int as Int does not have unique instances; have to wrap them in Newtype instances (ie Sum, Product)
- Only need to define Gen Arbitrary instances for polymorphic types (a, b, c etc).
Otherwise can just do:
arbitrary = <Data constructor> <$> arbitrary
- Type constraints are only used when types are unknown(polymorphic):
For example, 
-instance (Semigroup a, Semigroup b)=> Semigroup (Two a b) where
-instance Monoid a => Monoid (Identity a) where

```hs
-- 1.

data Trivial = Trivial deriving (Eq, Show)

instance Semigroup Trivial where
    (<>) Trivial _ = Trivial

instance Arbitrary Trivial where
    arbitrary = return Trivial

semigroupAssoc :: (Eq m, Semigroup m)
               => m -> m -> m -> Bool
semigroupAssoc a b c =
    (a <> (b <> c)) == ((a <> b) <> c)

type TrivAssoc =
  Trivial -> Trivial -> Trivial -> Bool

main :: IO ()  
main =  
    quickCheck (semigroupAssoc :: TrivAssoc) 

-- Just for fun:
genTrivial :: Gen Trivial
genTrivial = 
    return Trivial
```

2. newtype Identity a = Identity a
```hs
-- 2.

newtype Identity a = Identity a deriving (Eq, Show)

instance Semigroup a => Semigroup (Identity a) where
    (<>) (Identity x) (Identity y) = Identity (x <> y) 

genId :: Arbitrary a => Gen (Identity a)
genId = do
    a <- arbitrary
    return (Identity a)
instance Arbitrary a => Arbitrary (Identity a) where
    arbitrary = genId


semigroupAssoc :: (Eq m, Semigroup m)
               => m -> m -> m -> Bool
semigroupAssoc a b c =
    (a <> (b <> c)) == ((a <> b) <> c)


type IdType = Identity String
type IdAssoc =
    IdType -> IdType -> IdType -> Bool

main :: IO()
main = 
    quickCheck (semigroupAssoc :: IdAssoc)



--Just for fun:
genId :: Arbitrary a => Gen (Identity a)
genId = do
    a <- arbitrary
    return (Identity a)
instance Arbitrary a => Arbitrary (Identity a) where
    arbitrary = genId
identityGenInt :: Gen (Identity Int)
identityGenInt = genId
```

3. data Two a b = Two a b  
Hint: Ask for another Semigroup instance. 

```hs
-- 3.

data Two a b = Two a b deriving (Eq, Show)

instance (Semigroup a, Semigroup b) => Semigroup (Two a b) where
    (<>) (Two x y) (Two x' y') = Two (x <> x') (y <> y') 

genTwo :: (Arbitrary a, Arbitrary b) => Gen (Two a b)
genTwo = do
    a <- arbitrary
    b <- arbitrary
    return (Two a b) 

instance (Arbitrary a, Arbitrary b) => Arbitrary (Two a b) where
    arbitrary = genTwo

semigroupAssoc :: (Eq m, Semigroup m)
               => m -> m -> m -> Bool
semigroupAssoc a b c =
    (a <> (b <> c)) == ((a <> b) <> c)

type GenTwoType = Two String String
type GenTwoAssoc =
    GenTwoType -> GenTwoType -> GenTwoType -> Bool

main :: IO()
main = 
    quickCheck (semigroupAssoc :: GenTwoAssoc)
```


4. data Three a b c = Three a b c 
```hs
-- 4. 

data Three a b c = Three a b c deriving (Eq, Show)

instance (Semigroup a, Semigroup b, Semigroup c) => Semigroup (Three a b c) where
    (<>) (Three x y z) (Three x' y' z') = Three (x <> x') (y <> y') (z <> z') 

genThree :: (Arbitrary a, Arbitrary b, Arbitrary c) => Gen (Three a b c)
genThree = do
    a <- arbitrary
    b <-arbitrary
    c <-arbitrary
    return (Three a b c)

instance (Arbitrary a, Arbitrary b, Arbitrary c) => Arbitrary (Three a b c) where
    arbitrary = genThree

semigroupAssoc :: (Eq m, Semigroup m)
               => m -> m -> m -> Bool
semigroupAssoc a b c =
    (a <> (b <> c)) == ((a <> b) <> c)

type GenThreeType = Three String String String
type GenThreeAssoc = 
    GenThreeType -> GenThreeType -> GenThreeType -> Bool

main :: IO()
main = 
    quickCheck (semigroupAssoc :: GenThreeAssoc)
```

5. data Four a b c d = Four a b c d
```hs

-- 5.

data Four a b c d = Four a b c d deriving (Eq, Show)

instance (Semigroup a, Semigroup b, Semigroup c, Semigroup d) => Semigroup (Four a b c d) where
    (<>) (Four a b c d)(Four a' b' c' d') = Four (a <> a') (b <> b') (c <> c') (d <> d')

genFour :: (Arbitrary a, Arbitrary b, Arbitrary c, Arbitrary d) => Gen (Four a b c d)
genFour = do
    a <- arbitrary
    b <- arbitrary
    c <- arbitrary
    d <- arbitrary
    return (Four a b c d)
    
instance (Arbitrary a, Arbitrary b, Arbitrary c, Arbitrary d) => Arbitrary (Four a b c d) where
    arbitrary = genFour

semigroupAssoc :: (Eq m, Semigroup m)
               => m -> m -> m -> Bool
semigroupAssoc a b c =
    (a <> (b <> c)) == ((a <> b) <> c)

type GenFourType = Four String Ordering String [Bool]
type GenFourAssoc =
    GenFourType -> GenFourType -> GenFourType -> Bool

main :: IO()
main = 
    quickCheck (semigroupAssoc :: GenFourAssoc)
```

6. newtype BoolConj =  
BoolConj Bool  
What it should do:  
Prelude> (BoolConj True) <> (BoolConj True)  
BoolConj True  
Prelude> (BoolConj True) <> (BoolConj False)  
BoolConj False  
```hs
-- 6.

newtype BoolConj = 
    BoolConj Bool 
    deriving (Eq, Show)

instance Semigroup BoolConj where
    (<>) (BoolConj True) (BoolConj True) = BoolConj True
    (<>) _ _ = BoolConj False

instance Arbitrary BoolConj where
    arbitrary = do
    a <- arbitrary
    return (BoolConj a)

semigroupAssoc :: (Eq m, Semigroup m)
               => m -> m -> m -> Bool
semigroupAssoc a b c =
    (a <> (b <> c)) == ((a <> b) <> c)

type GenBoolConjAssoc =
    BoolConj -> BoolConj -> BoolConj -> Bool

main :: IO()
main =
    quickCheck (semigroupAssoc :: GenBoolConjAssoc)
```

7. newtype BoolDisj =  
BoolDisj Bool  
What it should do:  
Prelude> (BoolDisj True) <> (BoolDisj True)  
BoolDisj True  
Prelude> (BoolDisj True) <> (BoolDisj False)  
BoolDisj True  
```hs
-- 7.

newtype BoolDisj = 
    BoolDisj Bool 
    deriving (Eq, Show)

instance Semigroup BoolDisj where
    (<>) (BoolDisj False) (BoolDisj False) = BoolDisj False
    (<>) _ _ = BoolDisj True


instance Arbitrary BoolDisj where
    arbitrary = do
        a <- arbitrary
        return (BoolDisj a)

semigroupAssoc :: (Eq m, Semigroup m)
               => m -> m -> m -> Bool
semigroupAssoc a b c =
    (a <> (b <> c)) == ((a <> b) <> c)

type GenBoolDisjAssoc =
    BoolDisj -> BoolDisj -> BoolDisj -> Bool

main :: IO()
main =
    quickCheck (semigroupAssoc :: GenBoolDisjAssoc)
```

8. data Or a b =  
Fst a  
| Snd b  
The Semigroup for Or should have the following behavior.  
We can think of it as having a “sticky” Snd value, whereby it’ll hold onto the first Snd value when and if one is passed
as an argument. This is similar to the First' Monoid you wrote earlier:  

Prelude> Fst 1 <> Snd 2  
Snd 2  
Prelude> Fst 1 <> Fst 2  
Fst 2  
Prelude> Snd 1 <> Fst 2  
Snd 1  
Prelude> Snd 1 <> Snd 2  
Snd 1  
```hs
-- 8.
data Or a b =
    Fst a
  | Snd b
  deriving (Eq, Show)

instance Semigroup (Or a b) where
    (<>) (Fst _) x = x
    (<>) y _ = y


genOr :: (Arbitrary a, Arbitrary b) => Gen (Or a b)
genOr = do
    a <- arbitrary
    b <- arbitrary
    elements [Fst a, Snd b]

instance (Arbitrary a, Arbitrary b) => Arbitrary (Or a b) where
    arbitrary = genOr

semigroupAssoc :: (Eq m, Semigroup m)
               => m -> m -> m -> Bool
semigroupAssoc a b c =
    (a <> (b <> c)) == ((a <> b) <> c)

type OrTest = Or String String
type OrAssoc =
     OrTest-> OrTest -> OrTest -> Bool

main :: IO()
main =
    quickCheck (semigroupAssoc :: OrAssoc)
```

9. newtype Combine a b =  
Combine { unCombine :: (a -> b) }  
What it should do:  
Prelude> f = Combine $ \n -> Sum (n + 1)  
Prelude> g = Combine $ \n -> Sum (n - 1)  
Prelude> unCombine (f <> g) $ 0  
Sum {getSum = 0}  
Prelude> unCombine (f <> g) $ 1  
Sum {getSum = 2}  
Prelude> unCombine (f <> f) $ 1  
Sum {getSum = 4}  
Prelude> unCombine (g <> f) $ 1  
Sum {getSum = 2}  

Hint: This function will eventually be applied to a single value of type a. But you’ll have multiple functions that can
produce a value of type b. How do we combine multiple values so we have a single b? This one will probably be
tricky! Remember that the type of the value inside of Combine is that of a function. The type of functions should
already have an Arbitrary instance that you can reuse for testing this instance.  
```hs
-- 9.
newtype Combine a b =
    Combine { unCombine :: (a -> b) }

instance  Semigroup b => Semigroup (Combine a b) where
    (Combine { unCombine = f}) <> (Combine { unCombine = g}) = Combine $ \n -> f n <> g n

instance (CoArbitrary a, Arbitrary b) => Arbitrary (Combine a b) where
    arbitrary = do
        h <- arbitrary
        return $ Combine h 

semigroupAssoc :: (Eq m, Semigroup m)
               => m -> m -> m -> Bool
semigroupAssoc a b c =
    (a <> (b <> c)) == ((a <> b) <> c)

-- Can't seem to quickCheck the functions
```

10. newtype Comp a =  
Comp { unComp :: (a -> a) }  
Hint: We can do something that seems a little more specific and natural to functions now that the input and
output types are the same.  
```hs
-- 10.

newtype Comp a = 
    Comp { unComp :: (a -> a)}
    --deriving (Eq, Show a)

instance Semigroup a => Semigroup (Comp a) where
    (Comp {unComp = f1}) <> (Comp {unComp = f2}) = Comp $ f1 . f2

instance Arbitrary a => Arbitrary (Comp a) where
    arbitrary = do
        g <- arbitrary
        return (Comp g)

semigroupAssoc :: (Eq m, Semigroup m)
               => m -> m -> m -> Bool
semigroupAssoc a b c =
    (a <> (b <> c)) == ((a <> b) <> c)

type CompType = Comp (String -> Bool)
type CompAssoc =
    CompType -> CompType -> CompType -> Bool

main :: IO()
main = 
    quickCheck (semigroupAssoc :: CompAssoc)

-- Also can't quickCheck the function
```

11. Look familiar?  
data Validation a b =  
Failure a | Success b  
deriving (Eq, Show)  
instance Semigroup a =>  
Semigroup (Validation a b) where  
(<>) = undefined  
Given this code:  
main = do  
let failure :: String  
-> Validation String Int  
failure = Failure  
success :: Int  
-> Validation String Int  
success = Success  
print $ success 1 <> failure "blah"  
print $ failure "woot" <> failure "blah"  
print $ success 1 <> success 2  
print $ failure "woot" <> success 2  
You should get this output:  
Prelude> main  
Success 1  
Failure "wootblah"  
Success 1  
Success 2  
```hs
-- 11.

data Validation a b =
    Fail a | Pass b
    deriving (Eq, Show)

instance Semigroup a => 
  Semigroup (Validation a b ) where
      Pass x <> _ = Pass x
      Fail _ <> Pass y = Pass y
      Fail x <> Fail y = Fail $ x <> y

instance (Arbitrary a, Arbitrary b) => Arbitrary (Validation a b) where
    arbitrary = do
        x <- arbitrary
        y <- arbitrary
        elements [Pass x, Fail y]

semigroupAssoc :: (Eq m, Semigroup m)
               => m -> m -> m -> Bool
semigroupAssoc a b c =
    (a <> (b <> c)) == ((a <> b) <> c)

type ValTest = Validation String Int
type ValAssoc = ValTest -> ValTest -> ValTest -> Bool

main :: IO()
main = do
    --let failure :: String -> Validation String Int
        --failure = Failure
        --success :: Int -> Validation String Int
        --success = Success
        --print $ success 1 <> failure "blah"
        --print $ failure "woot" <> failure "blah"
        --print $ success 1 <> success 2
        --print $ failure "woot" <> success 2
    quickCheck (semigroupAssoc :: ValAssoc)
```

# Monoid exercises  
Given a datatype, implement the Monoid instance. Add Monoid constraints to type variables where needed. For the datatypes for which you’ve already implemented Semigroup instances, you need to figure out what the identity value is.  

1. Again, validate all of your instances with QuickCheck. Example scaffold is provided for the Trivial type:  
data Trivial = Trivial deriving (Eq, Show)  
instance Semigroup Trivial where  
(<>) = undefined  
instance Monoid Trivial where  
mempty = undefined  
mappend = (<>)  
type TrivAssoc =  
Trivial -> Trivial -> Trivial -> Bool  
main :: IO ()  
main = do  
let sa = semigroupAssoc  
mli = monoidLeftIdentity  
mlr = monoidRightIdentity  
quickCheck (sa :: TrivAssoc)  
quickCheck (mli :: Trivial -> Bool)  
quickCheck (mlr :: Trivial -> Bool)  
```hs
-- 1. 

data Trivial = Trivial deriving (Eq, Show)

instance Semigroup Trivial where
    (<>) Trivial _ = Trivial

instance Monoid Trivial where
    mempty = Trivial
    mappend = (<>)

instance Arbitrary Trivial where
    arbitrary = return Trivial

semigroupAssoc :: (Eq m, Semigroup m)
               => m -> m -> m -> Bool
semigroupAssoc a b c =
    (a <> (b <> c)) == ((a <> b) <> c)

type TrivAssoc = 
    Trivial -> Trivial -> Trivial -> Bool

main :: IO ()
main = do
  let sa = semigroupAssoc
      mli = monoidLeftIdentity
      mlr = monoidRightIdentity
  quickCheck (sa :: TrivAssoc)
  quickCheck (mli :: Trivial -> Bool)
  quickCheck (mlr :: Trivial -> Bool)
```

2. newtype Identity a =  
Identity a deriving Show  
```hs 
-- 2.
newtype Identity a = Identity a deriving (Eq, Show)

instance Semigroup a => Semigroup (Identity a) where
    (<>) (Identity x) (Identity y) = Identity (x <> y) 

instance Monoid a => Monoid (Identity a) where
    mempty = Identity mempty
    mappend = (<>)

genId :: Arbitrary a => Gen (Identity a)
genId = do
    a <- arbitrary
    return (Identity a)
instance Arbitrary a => Arbitrary (Identity a) where
    arbitrary = genId


semigroupAssoc :: (Eq m, Semigroup m)
               => m -> m -> m -> Bool
semigroupAssoc a b c =
    (a <> (b <> c)) == ((a <> b) <> c)


type IdType = Identity String
type IdAssoc =
    IdType -> IdType -> IdType -> Bool

main :: IO ()
main = do
  let sa = semigroupAssoc
      mli = monoidLeftIdentity
      mlr = monoidRightIdentity
  quickCheck (sa :: IdAssoc)
  quickCheck (mli :: IdType -> Bool)
  quickCheck (mlr :: IdType -> Bool)
```

3. data Two a b = Two a b deriving Show  
```hs
-- 3.

data Two a b = Two a b deriving (Eq, Show)

instance (Semigroup a, Semigroup b) => Semigroup (Two a b) where
    (<>) (Two x y) (Two x' y') = Two (x <> x') (y <> y') 

instance (Monoid a, Monoid b) => Monoid (Two a b) where
    mempty = Two mempty mempty


genTwo :: (Arbitrary a, Arbitrary b) => Gen (Two a b)
genTwo = do
    a <- arbitrary
    b <- arbitrary
    return (Two a b) 

instance (Arbitrary a, Arbitrary b) => Arbitrary (Two a b) where
    arbitrary = genTwo

semigroupAssoc :: (Eq m, Semigroup m)
               => m -> m -> m -> Bool
semigroupAssoc a b c =
    (a <> (b <> c)) == ((a <> b) <> c)

type GenTwoType = Two String String
type GenTwoAssoc =
    GenTwoType -> GenTwoType -> GenTwoType -> Bool

main :: IO ()
main = do
  let sa = semigroupAssoc
      mli = monoidLeftIdentity
      mlr = monoidRightIdentity
  quickCheck (sa :: GenTwoAssoc)
  quickCheck (mli :: GenTwoType -> Bool)
  quickCheck (mlr :: GenTwoType -> Bool)
```

4. newtype BoolConj =  
BoolConj Bool  
What it should do:  
Prelude> (BoolConj True) `mappend` mempty  
BoolConj True  
Prelude> mempty `mappend` (BoolConj False)  
BoolConj False  
```hs
-- 4.

newtype BoolConj = 
    BoolConj Bool 
    deriving (Eq, Show)

instance Semigroup BoolConj where
    (<>) (BoolConj True) (BoolConj True) = BoolConj True
    (<>) _ _ = BoolConj False

instance Monoid BoolConj where
    mempty = BoolConj True

instance Arbitrary BoolConj where
    arbitrary = do
    a <- arbitrary
    return (BoolConj a)

semigroupAssoc :: (Eq m, Semigroup m)
               => m -> m -> m -> Bool
semigroupAssoc a b c =
    (a <> (b <> c)) == ((a <> b) <> c)

type GenBoolConjAssoc =
    BoolConj -> BoolConj -> BoolConj -> Bool


main :: IO ()
main = do
  let sa = semigroupAssoc
      mli = monoidLeftIdentity
      mlr = monoidRightIdentity
  quickCheck (sa :: GenBoolConjAssoc)
  quickCheck (mli :: BoolConj -> Bool)
  quickCheck (mlr :: BoolConj -> Bool)
```

5. newtype BoolDisj =  
BoolDisj Bool  
What it should do:  
Prelude> (BoolDisj True) `mappend` mempty  
BoolDisj True  
Prelude> mempty `mappend` (BoolDisj False)  
BoolDisj False  
```hs
-- 5.

newtype BoolDisj = 
    BoolDisj Bool 
    deriving (Eq, Show)

instance Semigroup BoolDisj where
    (<>) (BoolDisj False) (BoolDisj False) = BoolDisj False
    (<>) _ _ = BoolDisj True

instance Monoid BoolDisj where
    mempty = BoolDisj False

instance Arbitrary BoolDisj where
    arbitrary = do
        a <- arbitrary
        return (BoolDisj a)

semigroupAssoc :: (Eq m, Semigroup m)
               => m -> m -> m -> Bool
semigroupAssoc a b c =
    (a <> (b <> c)) == ((a <> b) <> c)

type GenBoolDisjAssoc =
    BoolDisj -> BoolDisj -> BoolDisj -> Bool

main :: IO ()
main = do
  let sa = semigroupAssoc
      mli = monoidLeftIdentity
      mlr = monoidRightIdentity
  quickCheck (sa :: GenBoolDisjAssoc)
  quickCheck (mli :: BoolDisj -> Bool)
  quickCheck (mlr :: BoolDisj -> Bool)
```

6. newtype Combine a b =  
Combine { unCombine :: (a -> b) }  
What it should do:  
Prelude> f = Combine $ \n -> Sum (n + 1)  
Prelude> unCombine (mappend f mempty) $ 1  
Sum {getSum = 2}  
```hs
-- 6.
newtype Combine a b =
    Combine { unCombine :: (a -> b) }

instance  Semigroup b => Semigroup (Combine a b) where
    (Combine { unCombine = f}) <> (Combine { unCombine = g}) = Combine $ \n -> f n <> g n

instance Monoid b => Monoid (Combine a b) where
    mempty = Combine $ const mempty

instance (CoArbitrary a, Arbitrary b) => Arbitrary (Combine a b) where
    arbitrary = do
        h <- arbitrary
        return $ Combine h 

semigroupAssoc :: (Eq m, Semigroup m)
               => m -> m -> m -> Bool
semigroupAssoc a b c =
    (a <> (b <> c)) == ((a <> b) <> c)

-- Can't seem to quickCheck the functions
```

7. Hint: We can do something that seems a little more specific and natural to functions now that the input and output types are the same:  
newtype Comp a =  
Comp (a -> a)  
```hs
-- 7.
newtype Comp a = 
    Comp { unComp :: (a -> a)}
    --deriving (Eq, Show a)

instance Semigroup a => Semigroup (Comp a) where
    (Comp {unComp = f1}) <> (Comp {unComp = f2}) = Comp $ f1 . f2

instance Monoid (Comp a) where
    mempty = Comp id

instance Arbitrary a => Arbitrary (Comp a) where
    arbitrary = do
        g <- arbitrary
        return (Comp g)

semigroupAssoc :: (Eq m, Semigroup m)
               => m -> m -> m -> Bool
semigroupAssoc a b c =
    (a <> (b <> c)) == ((a <> b) <> c)

type CompType = Comp (String -> Bool)
type CompAssoc =
    CompType -> CompType -> CompType -> Bool

main :: IO()
main = 
    quickCheck (semigroupAssoc :: CompAssoc)

-- Also can't quickCheck the function
```

8. This next exercise will involve doing something that will still feel a bit unnatural, and you may find it difficult. If
you get it, and you haven’t done much FP or Haskell before, get yourself a nice beverage. We’re going to toss
you the instance declaration, so you don’t churn on a missing Monoid constraint you didn’t know you need:  
newtype Mem s a =  
Mem {  
runMem :: s -> (a,s)  
}  
instance Semigroup a => Semigroup (Mem s a) where  
(<>) = undefined  
instance Monoid a => Monoid (Mem s a) where  
mempty = undefined  
Given the following code:  
f' = Mem $ \s -> ("hi", s + 1)  
main = do  
let rmzero = runMem mempty 0  
rmleft = runMem (f' <> mempty) 0  
rmright = runMem (mempty <> f') 0  
print $ rmleft  
print $ rmright  
print $ (rmzero :: (String, Int))  
print $ rmleft == runMem f' 0  
print $ rmright == runMem f' 0  
A correct Monoid for Mem should, given the above code,  
produce the following output:  
Prelude> main  
("hi",1)  
("hi",1)  
("",0)  
True  
True  
Make certain your instance has output like the above, as this is sanity checking the Monoid identity laws for you! It’s
not a proof, and it’s not even as good as property testing, but it’ll catch the most common mistakes people make.
It’s not a trick, and you don’t need a Monoid for s. Yes, such a Monoid can and does exist. Hint: chain the s values from one function to the other. You’ll want to check the identity laws, as a common first attempt will break them.  
```hs
-- 8.

newtype Mem s a =
    Mem {
        runMem :: s -> (a,s)
    }

instance Semigroup a => Semigroup (Mem s a) where
    m1@(Mem f1) <> m2@(Mem f2) =
        Mem $ \s -> (fst (f1 s) <> fst (f2 s),
                     snd (f2 $ snd (f1 s)))

instance Monoid a => Monoid (Mem s a) where
    mempty = Mem $ \x -> (mempty, x)

type MemTest = Mem Int String
```