# Write map for BinaryTree
Given the definition of BinaryTree above, write a map function for the data structure. You don’t really need to know anything about binary trees to write these functions.  

The structure inherent in the definition of the type is all you need. All you need to do is write the recursive functions.  

No special algorithms are needed, and we don’t expect
you to keep the tree balanced or ordered. Also, remember
that we’ve never once mutated anything. We’ve only built new
values from input data. Given that, when you go to implement
mapTree, you’re not changing an existing tree—you’re building a new one based on an existing one (as when you are mapping functions over lists).  

<ins>Note, you do not need to use insert' for this.</ins>  

Retain the original structure of the tree:  
mapTree :: (a -> b)  
-> BinaryTree a  
-> BinaryTree b  
mapTree _ Leaf = Leaf  
mapTree f (Node left a right) =  
Node undefined undefined undefined  
testTree' :: BinaryTree Integer  
testTree' =  
Node (Node Leaf 3 Leaf)  
1  
(Node Leaf 4 Leaf)  
mapExpected =  
Node (Node Leaf 4 Leaf)  
2  
(Node Leaf 5 Leaf)  
-- acceptance test for mapTree  
mapOkay =  
if mapTree (+1) testTree' == mapExpected  
then print "yup OK!"  
else error "test failed!"  

Some hints for implementing mapTree follow.  
The first pattern match in our mapTree function is the base
case, where we have a Leaf value. We can’t apply the f there, because we don’t have an a, so we ignore it. Since we have to return a value of type BinaryTree b whatever happens, we return a Leaf value.  

We return a Node in the second pattern match of our mapTree
function. Note that the Node data constructor takes three arguments:  
Prelude> :t Node  
Node :: BinaryTree a  
-> a  
-> BinaryTree a  
-> BinaryTree a  

So, you need to pass it more BinaryTree, a single value, and
more BinaryTree. You have the following terms available to
you:  
1. f :: (a -> b)  
2. left :: BinaryTree a  
3. a :: a  
4. right :: BinaryTree a  

5. mapTree :: (a -> b)  
-> BinaryTree a  
-> BinaryTree b  

The Node returned needs to have a value of type b and
BinaryTree values with type a inside them. You have two functions at your disposal. One gets you (a -> b), the other maps BinaryTrees of type a into BinaryTrees of type b. Get ’em tiger.  

A few suggestions that might help you with this exercise:  
1. Split out the patterns your function should match on first.  
2. Implement the base case first.  
3. Try manually writing out the steps of recursion first, then collapse them into a single step that is recursive.  
Convert binary trees to lists  
Write functions to convert BinaryTree values to lists. Make
certain your implementation passes the tests:  
preorder :: BinaryTree a -> [a]  
preorder = undefined  
inorder :: BinaryTree a -> [a]  
inorder = undefined  

postorder :: BinaryTree a -> [a]  
postorder = undefined  
testTree :: BinaryTree Integer  
testTree =  
Node (Node Leaf 1 Leaf)  
2  
(Node Leaf 3 Leaf)  
testPreorder :: IO ()  
testPreorder =  
if preorder testTree == [2, 1, 3]  
then putStrLn "Preorder fine!"  
else putStrLn "Bad news bears."  

testInorder :: IO ()  
testInorder =  
if inorder testTree == [1, 2, 3]  
then putStrLn "Inorder fine!"  
else putStrLn "Bad news bears."  

testPostorder :: IO ()  
testPostorder =  
if postorder testTree == [1, 3, 2]  
then putStrLn "Postorder fine!"  
else putStrLn "Bad news bears"  

main :: IO ()  
main = do  
testPreorder  
testInorder  
testPostorder  
Write foldr for BinaryTree  

Given the definition of BinaryTree we have provided, write a
catamorphism for binary trees:  
-- any traversal order is fine  
foldTree :: (a -> b -> b)  
-> b  
-> BinaryTree a  
-> b  

```hs
data BinaryTree a = 
    Leaf
  | Node (BinaryTree a) a (BinaryTree a)
  deriving (Eq, Ord, Show)

insert' :: Ord a
        => a
        -> BinaryTree a
        -> BinaryTree a

insert' b Leaf = Node Leaf b Leaf
insert' b (Node left a right)
  | b == a = Node left a right
  | b < a = Node (insert' b left) a right
  | b > a = Node left a (insert' b right)

mapTree :: (a -> b)
        -> BinaryTree a
        -> BinaryTree b
mapTree _ Leaf = Leaf
mapTree f (Node left a right) = 
    Node undefined undefined undefined

testTree' :: BinaryTree Integer
testTree' =
    Node (Node Leaf 3 Leaf)
         1
         (Node Leaf 4 Leaf)

mapExpected = 
    Node (Node Leaf 4 Leaf)
         2
         (Node Leaf 5 Leaf)

mapOkay = 
    if mapTree (+1) testTree' == mapExpected
        then print "yup OK!"
        else error "test failed!"

mapTree' :: (a -> b) -> BinaryTree a -> BinaryTree b
mapTree' _ Leaf = Leaf
mapTree' f (Node left x right) = 
    Node (mapTree f left) (f x) (mapTree f right) 

testTree :: BinaryTree Integer
testTree = 
    Node (Node Leaf 1 Leaf)
         2
         (Node Leaf 3 Leaf)

preorder :: BinaryTree a -> [a]
preorder Leaf = []
preorder (Node left x right) = 
    [x] ++ preorder left ++ preorder right
testPreorder :: IO()
testPreorder =
    if preorder testTree == [2,1,3]
        then putStrLn "Preorder fine!"
        else putStrLn "Bad news bears"

inorder :: BinaryTree a -> [a]
inorder Leaf = []
inorder (Node left y right) = 
    inorder left ++ [y] ++ inorder right
testInorder :: IO()
testInorder = 
    if inorder testTree == [1, 2, 3]
        then putStrLn "Inorder fine!"
        else putStrLn "Bad news bears."

postorder :: BinaryTree a -> [a]
postorder Leaf = []
postorder (Node left z right) = 
    postorder left ++ postorder right ++ [z]

testPostorder :: IO()
testPostorder = 
    if postorder testTree == [1, 3, 2]
    then putStrLn "Postorder fine!"
    else putStrLn "Bad news bears"

main :: IO()
main = do
    testPreorder
    testInorder
    testPostorder

--Write foldr for BinaryTree

--any traversal order is fine
foldTree :: (a -> b-> b)
          -> b
          -> BinaryTree a
          -> b
foldTree Leaf = Node (BinaryTree a) a (BinaryTree a)
```